Made MultiRound invariant inductive across Accept, making use of no packet duplication

ironfleet/src/Dafny/Distributed/Protocol/Lock/PerformanceProof/MultiRoundPerformanceProof.i.dfy
@@ -1,17 +1,38 @@
-include "../../../Services/Lock/LockTaggedDistributedSystem.i.dfy"
-include "TaggedGLS.i.dfy"
-include "Definitions_arith.i.dfy"
+include "../../../Services/Lock/LockTimestampedDistributedSystem.i.dfy"
+include "TimestampedGLS_noduplication.i.dfy"
+include "Definitions.i.dfy"
 include "../../../../Libraries/Math/mod_auto.i.dfy"
+include "MultiRoundTimeHelpers.i.dfy"
+include "../../../Common/Collections/Multisets.s.dfy"
 
 module MultiRoundPerformanceProof_i {
 
-import opened LockTaggedDistributedSystem_i
-  import opened TaggedGLS_i
+import opened LockTimestampedDistributedSystem_i
+  import opened TimestampedGLS_noduplication_i
   import opened PerformanceProof__Definitions_i
   import opened Math__mod_auto_i
+  import opened PerformanceProof__MultiRoundTimeHelpers_i
+  import opened Collections__Multisets_s
 
-predicate {:verify false} SingleGLSPerformanceAssumption(tgls:TaggedGLS_State)
+predicate NoPacketDuplication(tls:TimestampedLS_State)
 {
+  var nextStep := tls.t_environment.nextStep;
+  nextStep.LEnvStepHostIos? ==> (
+  (forall io :: io in nextStep.ios && io.LIoOpReceive? ==> io.r in tls.undeliveredPackets)
+  )
+}
+
+predicate LockedPacketNeverDelivered(tls:TimestampedLS_State)
+{
+  var nextStep := tls.t_environment.nextStep;
+  nextStep.LEnvStepHostIos? ==> (forall io :: io in nextStep.ios && io.LIoOpReceive? ==> !io.r.msg.v.Locked?)
+}
+
+predicate SingleGLSPerformanceAssumption(tgls:TimestampedGLS_State)
+{
+  && NoPacketDuplication(tgls.tls)
+  && LockedPacketNeverDelivered(tgls.tls)
+
   // The only nodes that take steps are in the ring
   && (tgls.tls.t_environment.nextStep.LEnvStepHostIos? ==> tgls.tls.t_environment.nextStep.actor in tgls.tls.t_servers)
 
@@ -32,44 +53,60 @@ predicate {:verify false} SingleGLSPerformanceAssumption(tgls:TaggedGLS_State)
 
 }
 
-predicate {:verify false} GLSPerformanceAssumption(tglb:seq<TaggedGLS_State>)
+predicate GLSPerformanceAssumption(tglb:seq<TimestampedGLS_State>)
 {
   forall tgls :: tgls in tglb ==> SingleGLSPerformanceAssumption(tgls)
 }
 
-predicate {:verify false} SingleGLSPerformanceGuarantee(gls:TaggedGLS_State)
+predicate SingleGLSPerformanceGuarantee(gls:TimestampedGLS_State)
 {
   |gls.tls.config| > 1 ==> 
   (forall pkt :: pkt in gls.tls.t_environment.sentPackets &&
-    pkt.msg.v.Transfer? ==> pkt.msg.v.transfer_epoch > 1 && PerfLe(pkt.msg.pr, PerfBoundLockInNetwork(pkt.msg.v.transfer_epoch)))
+    pkt.msg.v.Transfer? ==> pkt.msg.v.transfer_epoch > 1 && TimeLe(pkt.msg.ts, PerfBoundLockInNetwork(pkt.msg.v.transfer_epoch)))
 }
 
-predicate {:verify false} GLSPerformanceGuarantee(tglb:seq<TaggedGLS_State>)
+predicate GLSPerformanceGuarantee(tglb:seq<TimestampedGLS_State>)
 {
   forall tgls :: tgls in tglb ==> SingleGLSPerformanceGuarantee(tgls)
 }
 
-predicate {:verify false} TGLS_Consistency(tgls: TaggedGLS_State)
+predicate TGLS_Consistency(tgls: TimestampedGLS_State)
 {
   && (forall id :: id in tgls.tls.config <==> id in tgls.tls.t_servers)
     && (forall id :: id in tgls.tls.t_servers ==> (tgls.tls.t_servers[id].v.config == tgls.tls.config))
     && (forall i :: 0 <= i < |tgls.tls.config| ==> tgls.tls.t_servers[tgls.tls.config[i]].v.my_index == i)
 }
 
-predicate PerfInvariantAlways_NodeNotHeld(tgls:TaggedGLS_State, t_hs:TaggedType<Node>)
+predicate NoTransferPacketsToId(config:ConcreteConfiguration, pkts:multiset<TimestampedLPacket<EndPoint, LockMessage>>, id:EndPoint)
+  // ensures forall pkt :: !pkt.Transfer? ==>
 {
-  // || (forall pkt in env.sentPackets )
-    || (false)
+  (forall pkt :: pkt in pkts && pkt.msg.v.Transfer? && pkt.dst == id && pkt.src in config ==> false)
 }
 
-predicate PerfInvariantAlways_Node(t_hs:TaggedType<Node>)
+predicate PerfInvariantAlways_Node(tgls:TimestampedGLS_State, id:EndPoint)
+  requires id in tgls.tls.t_servers
 {
+  var t_hs := tgls.tls.t_servers[id];
+  (
   && (t_hs.v.epoch >= 0)
-  && (t_hs.v.held == false ==> t_hs.v.epoch > 0 && PerfLe(t_hs.pr, PerfBoundLockInNetwork(t_hs.v.epoch + 1)))
-  && (t_hs.v.held == true  ==> t_hs.v.epoch > 0 && PerfLe(t_hs.pr, PerfBoundLockHeld(t_hs.v.epoch)))
+  && (t_hs.v.held == false ==> t_hs.v.epoch > 0 && TimeLe(t_hs.ts, PerfBoundLockInNetwork(t_hs.v.epoch + 1)))
+  && (t_hs.v.held == true  ==> t_hs.v.epoch > 0 && TimeLe(t_hs.ts, PerfBoundLockHeld(t_hs.v.epoch)))
+  )
+
+  && (
+  if t_hs.v.held then
+    NoTransferPacketsToId(tgls.tls.config, tgls.tls.undeliveredPackets, id)
+  else
+     (forall pkt :: pkt in tgls.tls.undeliveredPackets && pkt.msg.v.Transfer? && pkt.dst == id && pkt.src in tgls.tls.t_servers ==>
+     (var undeliveredPackets' := tgls.tls.undeliveredPackets - multiset({pkt});
+        NoTransferPacketsToId(tgls.tls.config, undeliveredPackets', id)
+        )
+
+    )
+  )
 }
 
-predicate {:verify false} PerfInvariantAlways(tgls:TaggedGLS_State)
+predicate PerfInvariantAlways(tgls:TimestampedGLS_State)
   requires TGLS_Consistency(tgls)
 {
   // No irrelevant packets in sentPackets
@@ -79,429 +116,84 @@ predicate {:verify false} PerfInvariantAlways(tgls:TaggedGLS_State)
   // No nodes with epoch higher
   &&  (forall id :: id in tgls.tls.t_servers ==> 0 <= tgls.tls.t_servers[id].v.epoch <= |tgls.history|)
 
+  // No Invalid packets are ever sent
+  && (forall pkt :: pkt in tgls.tls.undeliveredPackets
+  ==>
+  !pkt.msg.v.Invalid?)
+
   // No transfer packets with epoch higher than history size
   // All transfer packets have correct performance object, determined by its transfer_epoch
-  && (forall pkt :: pkt in tgls.tls.t_environment.sentPackets && pkt.msg.v.Transfer? && pkt.dst in tgls.tls.t_servers && pkt.src in tgls.tls.t_servers
-  ==> 0 < pkt.msg.v.transfer_epoch ) // <= |tgls.history|)
+  // All undelivered transfer packets are acceptable
+  && (forall pkt :: pkt in tgls.tls.undeliveredPackets && pkt.msg.v.Transfer? && pkt.dst in tgls.tls.t_servers
+  ==> && pkt.src in tgls.tls.t_servers
+  && 1 < pkt.msg.v.transfer_epoch <= |tgls.history| && TimeLe(pkt.msg.ts, PerfBoundLockInNetwork(pkt.msg.v.transfer_epoch))
+  && pkt.msg.v.transfer_epoch > tgls.tls.t_servers[pkt.dst].v.epoch
+  )
 
-  && (forall pkt :: pkt in tgls.tls.t_environment.sentPackets && pkt.msg.v.Locked? && pkt.dst in tgls.tls.t_servers && pkt.src in tgls.tls.t_servers
-  ==> 0 < pkt.msg.v.locked_epoch ) // <= |tgls.history|)
-
-  && ( forall pkt :: pkt in tgls.tls.t_environment.sentPackets && pkt.msg.v.Transfer? && pkt.dst in tgls.tls.t_servers && pkt.src in tgls.tls.t_servers
-  ==> pkt.msg.v.transfer_epoch > 1 && PerfLe(pkt.msg.pr, PerfBoundLockInNetwork(pkt.msg.v.transfer_epoch)))
-
-  && ( forall pkt :: pkt in tgls.tls.t_environment.sentPackets && pkt.msg.v.Locked? && pkt.dst in tgls.tls.t_servers && pkt.src in tgls.tls.t_servers
-  ==> pkt.msg.v.locked_epoch > 1 && PerfLe(pkt.msg.pr, PerfBoundLockHeld(pkt.msg.v.locked_epoch)))
-
-  && (forall id :: id in tgls.tls.t_servers ==> PerfInvariantAlways_Node(tgls.tls.t_servers[id]))
+  && (forall id :: id in tgls.tls.t_servers ==> PerfInvariantAlways_Node(tgls, id))
 }
 
-predicate {:verify false} PerfInvariantLockHeld(tgls: TaggedGLS_State, j:int, epoch:int)
-  requires 0 < epoch
-  requires 0 <= j < |tgls.tls.config|
-  requires TGLS_Consistency(tgls)
-{
-  && PerfInvariantAlways(tgls)
-  && SingleGLSPerformanceGuarantee(tgls)
-  && tgls.tls.t_servers[tgls.tls.config[j]].v.held == true
-  && |tgls.history| == epoch
-  && tgls.tls.t_servers[tgls.tls.config[j]].v.epoch == |tgls.history|
-  && j == (epoch - 1) % |tgls.tls.config|
 
-  && ( forall pkt :: pkt in tgls.tls.t_environment.sentPackets && pkt.msg.v.Transfer? && pkt.dst in tgls.tls.t_servers && pkt.src in tgls.tls.t_servers
-  ==> && pkt.msg.v.transfer_epoch > 1 && PerfLe(pkt.msg.pr, PerfBoundLockInNetwork(pkt.msg.v.transfer_epoch)))
-
-  && ( forall pkt :: pkt in tgls.tls.t_environment.sentPackets && pkt.msg.v.Locked? && pkt.dst in tgls.tls.t_servers && pkt.src in tgls.tls.t_servers
-  ==> pkt.msg.v.locked_epoch > 1 && PerfLe(pkt.msg.pr, PerfBoundLockHeld(pkt.msg.v.locked_epoch)))
-
-  && (forall id :: id in tgls.tls.t_servers && tgls.tls.t_servers[id].v.held == true ==> PerfLe(tgls.tls.t_servers[id].pr, PerfBoundLockHeld(tgls.tls.t_servers[id].v.epoch)) )
-  // && (forall id :: id in tgls.tls.t_servers && tgls.tls.t_servers[id].v.held == false ==> PerfLe(tgls.tls.t_servers[id].pr, tgls.tls.t_servers[id].v.epoch) )
-
-
-  &&  (forall id :: id in tgls.tls.t_servers && id != tgls.tls.config[j]
-  ==> tgls.tls.t_servers[id].v.held == false && tgls.tls.t_servers[id].v.epoch < |tgls.history|)
-
-  // The node with the lock has correct PerfReport
-  && PerfEq(tgls.tls.t_servers[tgls.tls.config[j]].pr, PerfBoundLockHeld(epoch))
-}
-
-predicate {:verify false} PerfInvariantLockInNetwork(tgls: TaggedGLS_State, j:int, epoch:int)
-  requires 1 < epoch
-  requires 0 <= j < |tgls.tls.config|
-  requires TGLS_Consistency(tgls)
-{
-  && PerfInvariantAlways(tgls)
-  && SingleGLSPerformanceGuarantee(tgls)
-  && |tgls.history| == epoch
-  && j == (epoch - 1) % |tgls.tls.config|
-
-
-  && ( forall pkt :: pkt in tgls.tls.t_environment.sentPackets && pkt.msg.v.Transfer? && pkt.dst in tgls.tls.t_servers && pkt.src in tgls.tls.t_servers
-  ==> pkt.msg.v.transfer_epoch > 1 && PerfLe(pkt.msg.pr, PerfBoundLockInNetwork(pkt.msg.v.transfer_epoch)))
-
-  && ( forall pkt :: pkt in tgls.tls.t_environment.sentPackets && pkt.msg.v.Locked? && pkt.dst in tgls.tls.t_servers && pkt.src in tgls.tls.t_servers
-  ==> pkt.msg.v.locked_epoch > 1 && PerfLe(pkt.msg.pr, PerfBoundLockHeld(pkt.msg.v.locked_epoch)))
-
-  && (forall id :: id in tgls.tls.t_servers && tgls.tls.t_servers[id].v.held == true ==> PerfLe(tgls.tls.t_servers[id].pr, PerfBoundLockHeld(tgls.tls.t_servers[id].v.epoch)) )
-  // && (forall id :: id in tgls.tls.t_servers && tgls.tls.t_servers[id].v.held == false ==> PerfLe(tgls.tls.t_servers[id].pr, tgls.tls.t_servers[id].v.epoch) )
-
-
-  // No one holds the lock; everyone's epoch is below the epoch of the newest packet.
-  && (forall id :: id in tgls.tls.t_servers ==> tgls.tls.t_servers[id].v.held == false && tgls.tls.t_servers[id].v.epoch < |tgls.history|)
-
-  && ( forall pkt :: pkt in tgls.tls.t_environment.sentPackets && pkt.msg.v.Transfer? && pkt.dst in tgls.tls.t_servers && pkt.src in tgls.tls.t_servers
-      && pkt.msg.v.transfer_epoch == |tgls.history|
-      ==> pkt.dst == tgls.tls.config[j] && pkt.src == tgls.tls.config[(j - 1) % |tgls.tls.config|] && PerfEq(pkt.msg.pr, PerfBoundLockInNetwork(epoch)))
-
-}
-
-lemma Grant_InvImpliesInv(s:TaggedGLS_State, s':TaggedGLS_State)
+lemma Grant_j_InvLockHeldImpliesInvLockHeld(j:int, s:TimestampedGLS_State, s':TimestampedGLS_State)
   requires TGLS_Next(s, s')
+  requires 0 <= j < |s.tls.config|
   requires TGLS_Consistency(s) && TGLS_Consistency(s')
   requires SingleGLSPerformanceAssumption(s)
-  requires SingleGLSPerformanceAssumption(s')
 
   // A node other than node j taking a grant step
   requires s.tls.t_environment.nextStep.LEnvStepHostIos?
+  requires s.tls.t_environment.nextStep.actor == s.tls.config[j]
   requires s.tls.t_environment.nextStep.nodeStep == GrantStep
-  requires s.tls.t_servers[s.tls.t_environment.nextStep.actor].v.held == true
 
   requires PerfInvariantAlways(s);
   ensures PerfInvariantAlways(s');
 {
-  lemma_mod_auto(|s.tls.config|);
-  var step := s.tls.t_environment.nextStep;
-  var id := step.actor;
-  var pkt := step.ios[0].s;
-  var epoch := s.tls.t_servers[id].v.epoch;
-  var node_pr := s.tls.t_servers[id].pr;
-  // assert node_pr == PerfBoundLockHeld(epoch);
-  lemma_Grant(node_pr, epoch);
-  assert PerfInvariantAlways_Node(s'.tls.t_servers[id]);
+  var t_hs := s.tls.t_servers[s.tls.config[j]];
+  lemma_Grant(t_hs.ts, t_hs.v.epoch);
+  assert PerfInvariantAlways_Node(s', s.tls.config[j]);
+  // assert forall id :: id in s.tls.t_servers ==> PerfInvariant
 }
 
-lemma Accept_InvImpliesInv(s:TaggedGLS_State, s':TaggedGLS_State)
+lemma Accept_j_InvLockHeldImpliesInvLockHeld(j:int, s:TimestampedGLS_State, s':TimestampedGLS_State)
   requires TGLS_Next(s, s')
+  requires 0 <= j < |s.tls.config|
   requires TGLS_Consistency(s) && TGLS_Consistency(s')
   requires SingleGLSPerformanceAssumption(s)
-  requires SingleGLSPerformanceAssumption(s')
-
-  // A node other than node j taking a grant step
-  requires s.tls.t_environment.nextStep.LEnvStepHostIos?
-  requires s.tls.t_environment.nextStep.nodeStep == AcceptStep
-  // requires s.tls.t_servers[s.tls.t_environment.nextStep.actor].v.held == true
-
-  requires PerfInvariantAlways(s);
-  ensures PerfInvariantAlways(s');
-{
-  lemma_mod_auto(|s.tls.config|);
-  var step := s.tls.t_environment.nextStep;
-  var id := step.actor;
-  var ios := step.ios;
-  var pkt := ios[0].r;
-  var epoch := s.tls.t_servers[id].v.epoch;
-  var node_pr := s.tls.t_servers[id].pr;
-  assert pkt.msg.v.Transfer?;
-
-  if (pkt.msg.v.transfer_epoch > s.tls.t_servers[id].v.epoch) {
-    assert PerfInvariantAlways(s');
-  }
-}
-
-lemma {:verify false} NotHostIos_InvLockHeldImpliesInvLockHeld(j:int, epoch:int, s:TaggedGLS_State, s':TaggedGLS_State)
-  requires TGLS_Next(s, s')
-  requires 0 <= j < |s.tls.config|
-  requires 0 < epoch
-  requires TGLS_Consistency(s) && TGLS_Consistency(s')
-
-  // Not a HostIos step
-  requires !s.tls.t_environment.nextStep.LEnvStepHostIos?
-
-  requires PerfInvariantLockHeld(s, j, epoch);
-  ensures PerfInvariantLockHeld(s', j, epoch);
-{
-  //reveal_PerfInvariantLockHeld();
-}
-
-lemma {:verify false} Grant_not_j_InvLockHeldImpliesInvLockHeld(j:int, epoch:int, s:TaggedGLS_State, s':TaggedGLS_State)
-  requires TGLS_Next(s, s')
-  requires 0 <= j < |s.tls.config|
-  requires j == (epoch - 1) % |s.tls.config|
-  requires 0 < epoch
-  requires TGLS_Consistency(s) && TGLS_Consistency(s')
-  requires SingleGLSPerformanceAssumption(s)
-
-  // A node other than node j taking a grant step
-  requires s.tls.t_environment.nextStep.LEnvStepHostIos?
-  requires s.tls.t_environment.nextStep.actor != s.tls.config[j]
-  requires s.tls.t_environment.nextStep.nodeStep == GrantStep
-
-  requires PerfInvariantLockHeld(s, j, epoch);
-  ensures PerfInvariantLockHeld(s', j, epoch);
-{
-  lemma_mod_auto(|s.tls.config|);
-  //reveal_PerfInvariantLockHeld();
-}
-
-lemma {:verify false} Accept_not_j_InvLockHeldImpliesInvLockHeld(j:int, epoch:int, s:TaggedGLS_State, s':TaggedGLS_State)
-  requires TGLS_Next(s, s')
-  requires 0 <= j < |s.tls.config|
-  requires 0 < epoch
-  requires j == (epoch - 1) % |s.tls.config|
-
-  requires TGLS_Consistency(s) && TGLS_Consistency(s')
-  requires SingleGLSPerformanceAssumption(s)
-
-  // A node other than node j taking an accept step
-  requires s.tls.t_environment.nextStep.LEnvStepHostIos?
-  requires s.tls.t_environment.nextStep.actor != s.tls.config[j]
-  requires s.tls.t_environment.nextStep.nodeStep == AcceptStep
-
-  requires PerfInvariantLockHeld(s, j, epoch);
-  ensures PerfInvariantLockHeld(s', j, epoch);
-{
-  lemma_mod_auto(|s.tls.config|);
-  // assert false;
-  //reveal_PerfInvariantLockHeld();
-}
-
-lemma {:verify false} Grant_j_InvLockHeldImpliesInvLockInNetwork(j:int, epoch:int, s:TaggedGLS_State, s':TaggedGLS_State)
-  requires TGLS_Next(s, s')
-  requires 0 <= j < |s.tls.config|
-  requires 0 < epoch
-  requires j == (epoch - 1) % |s.tls.config|
-  
-  requires TGLS_Consistency(s) && TGLS_Consistency(s')
-  requires SingleGLSPerformanceAssumption(s)
-  requires SingleGLSPerformanceAssumption(s')
-
-  // A node other than node j taking a grant step
-  requires s.tls.t_environment.nextStep.LEnvStepHostIos?
-  // requires s.tls.t_environment.nextStep.actor == s.tls.config[j]
-  requires s.tls.t_environment.nextStep.nodeStep == GrantStep
-
-  requires PerfInvariantLockHeld(s, j, epoch);
-  ensures PerfInvariantLockInNetwork(s', (j + 1) % |s.tls.config|, epoch + 1);
-{
-  //reveal_PerfInvariantLockHeld();
-  //reveal_PerfInvariantLockInNetwork();
-  assert false;
-
-  lemma_mod_auto(|s.tls.config|);
-  //PerfProperties();
-  //var p := PerfBoundLockHeld(epoch);
-  //var p' := PerfBoundLockInNetwork(epoch + 1);
-  //assert PerfEq(p', PerfAdd2(p, PerfStep(GrantStep)));
-}
-
-lemma {:verify false} NotHostIos_InvLockInNetworkImpliesInvLockInNetwork(j:int, epoch:int, s:TaggedGLS_State, s':TaggedGLS_State)
-  requires TGLS_Next(s, s')
-  requires 0 <= j < |s.tls.config|
-  requires 1 < epoch
-  requires j == (epoch - 1) % |s.tls.config|
-
-  requires TGLS_Consistency(s) && TGLS_Consistency(s')
-
-  // Not a HostIos step
-  requires !s.tls.t_environment.nextStep.LEnvStepHostIos?
-
-  requires PerfInvariantLockInNetwork(s, j, epoch);
-  ensures PerfInvariantLockInNetwork(s', j, epoch);
-{
-  //reveal_PerfInvariantLockInNetwork();
-}
-
-lemma {:verify false} Accept_not_j_InvLockInNetworkImpliesInvLockInNetwork(j:int, epoch:int, s:TaggedGLS_State, s':TaggedGLS_State)
-  requires TGLS_Next(s, s')
-  requires 0 <= j < |s.tls.config|
-  requires 1 < epoch
-  requires j == (epoch - 1) % |s.tls.config|
-
-  requires TGLS_Consistency(s) && TGLS_Consistency(s')
-  requires SingleGLSPerformanceAssumption(s)
-  requires SingleGLSPerformanceAssumption(s')
-
-  // A node other than node j taking a grant step
-  requires s.tls.t_environment.nextStep.LEnvStepHostIos?
-  requires s.tls.t_environment.nextStep.actor != s.tls.config[j]
-  requires s.tls.t_environment.nextStep.nodeStep == AcceptStep
-
-  requires PerfInvariantLockInNetwork(s, j, epoch);
-  ensures PerfInvariantLockInNetwork(s', j, epoch);
-{
-  //reveal_PerfInvariantLockInNetwork();
-
-  lemma_mod_auto(|s.tls.config|);
-}
-
-lemma {:verify false} Accept_j_InvLockInNetworkImpliesInvLockHeld(j:int, epoch:int, s:TaggedGLS_State, s':TaggedGLS_State)
-  requires TGLS_Next(s, s')
-  requires 0 <= j < |s.tls.config|
-  requires 1 < epoch
-  requires j == (epoch - 1) % |s.tls.config|
-
-  requires TGLS_Consistency(s) && TGLS_Consistency(s')
-  requires SingleGLSPerformanceAssumption(s)
-  requires SingleGLSPerformanceAssumption(s')
 
   // A node other than node j taking a grant step
   requires s.tls.t_environment.nextStep.LEnvStepHostIos?
   requires s.tls.t_environment.nextStep.actor == s.tls.config[j]
   requires s.tls.t_environment.nextStep.nodeStep == AcceptStep
 
-  requires PerfInvariantLockInNetwork(s, j, epoch);
-  ensures PerfInvariantLockHeld(s', j, epoch);
+  requires PerfInvariantAlways(s);
+  ensures PerfInvariantAlways(s');
 {
-  //reveal_PerfInvariantLockInNetwork();
-  //reveal_PerfInvariantLockHeld();
-  //PerfProperties();
-
-  lemma_mod_auto(|s.tls.config|);
-}
-
-lemma {:verify false} PerfInvariantLockInNetworkGoesToPerfInvariant(j:int, epoch:int, s:TaggedGLS_State, s':TaggedGLS_State)
-  requires SingleGLSPerformanceAssumption(s) && TGLS_Consistency(s)
-  requires SingleGLSPerformanceAssumption(s') && TGLS_Consistency(s')
-  requires TGLS_Next(s, s')
-  requires 0 <= j < |s.tls.config|
-  requires 1 < epoch
-  requires j == (epoch - 1) % |s.tls.config|
-
-  requires 1 < epoch <= |s.tls.config|
-  requires PerfInvariantLockInNetwork(s, j, epoch)
-
-  ensures PerfInvariant(s')
-{
-  if !s.tls.t_environment.nextStep.LEnvStepHostIos? {
-    NotHostIos_InvLockInNetworkImpliesInvLockInNetwork(j, epoch, s, s');
-  } else {
-    if s.tls.t_environment.nextStep.actor == s.tls.config[j] {
-      if s.tls.t_environment.nextStep.nodeStep == GrantStep {
-        //reveal_PerfInvariantLockInNetwork();
-        assert false;
-      } else {
-        Accept_j_InvLockInNetworkImpliesInvLockHeld(j, epoch, s, s');
-      }
-    } else {
-      if s.tls.t_environment.nextStep.nodeStep == GrantStep {
-        //reveal_PerfInvariantLockInNetwork();
-        // assert false;
-      } else {
-        // Accept_not_j_InvLockInNetworkImpliesInvLockInNetwork(j, epoch, s, s');
-      }
-    }
+  var t_hs := s.tls.t_servers[s.tls.config[j]];
+  // lemma_Grant(t_hs.ts, t_hs.v.epoch);
+  var ios := s.tls.t_environment.nextStep.ios;
+  var id := s.tls.t_environment.nextStep.actor;
+  assert IsValidLIoOp(ios[0], id, s.tls.t_environment);
+  var pkt := ios[0].r;
+  assert pkt in s.tls.undeliveredPackets;
+  match pkt.msg.v {
+    case Locked(_) =>
+      assert false;
+    case Transfer(_) =>
+      assert pkt.msg.v.Transfer?;
   }
+  assert !(pkt.msg.v.Locked?);
+  assert pkt.msg.v.Transfer?;
+  assert s'.tls.t_servers[s.tls.config[j]].v.held == true;
+  var undeliveredPackets' := s.tls.undeliveredPackets - multiset{pkt};
+  var s_pkt := ios[1].s;
+  assert !s_pkt.msg.v.Transfer?;
+  assert NoTransferPacketsToId(s.tls.config, undeliveredPackets', id);
+  assert s'.tls.undeliveredPackets == undeliveredPackets' + multiset{s_pkt};
+  assert NoTransferPacketsToId(s.tls.config, s'.tls.undeliveredPackets, id);
+  lemma_Accept(s.tls.t_servers[id].ts, pkt.msg.ts, s.tls.t_servers[id].v.epoch, pkt.msg.v.transfer_epoch);
+
+  assert PerfInvariantAlways_Node(s', s.tls.config[j]);
 }
 
-////////////////////////////////////////////////////////////////////////////////
-
-predicate {:verify false} PerfInvariant(tgls:TaggedGLS_State)
-{
-  && TGLS_Consistency(tgls)
-  && ( 
-    || (exists epoch, j :: 0 < epoch && j == (epoch - 1) % |tgls.tls.config| && 0 <= j < |tgls.tls.config| && PerfInvariantLockHeld(tgls, j, epoch))
-    || (exists epoch, j :: 1 < epoch && j == (epoch - 1) % |tgls.tls.config| && 0 <= j < |tgls.tls.config| && PerfInvariantLockInNetwork(tgls, j, epoch))
-  )
-}
-
-lemma {:verify false} PerfInvariantLockHeldGoesToPerfInvariant(j:int, epoch:int, s:TaggedGLS_State, s':TaggedGLS_State)
-  requires SingleGLSPerformanceAssumption(s) && TGLS_Consistency(s)
-  requires SingleGLSPerformanceAssumption(s') && TGLS_Consistency(s')
-  requires TGLS_Next(s, s')
-  requires 0 <= j < |s.tls.config|
-  requires 0 < epoch
-  requires j == (epoch - 1) % |s.tls.config|
-  requires PerfInvariantLockHeld(s, j, epoch)
-
-  ensures PerfInvariant(s')
-{
-  lemma_mod_auto(|s.tls.config|);
-  if !s.tls.t_environment.nextStep.LEnvStepHostIos? {
-    NotHostIos_InvLockHeldImpliesInvLockHeld(j, epoch, s, s');
-  } else {
-    if s.tls.t_environment.nextStep.actor == s.tls.config[j] {
-      if s.tls.t_environment.nextStep.nodeStep == GrantStep {
-        Grant_j_InvLockHeldImpliesInvLockInNetwork(j, epoch, s, s');
-      } else {
-        assert false;
-      }
-    } else {
-      if s.tls.t_environment.nextStep.nodeStep == GrantStep {
-        Grant_not_j_InvLockHeldImpliesInvLockHeld(j, epoch, s, s');
-      } else {
-        Accept_not_j_InvLockHeldImpliesInvLockHeld(j, epoch, s, s');
-      }
-    }
-  }
-}
-
-lemma {:verify false} PerfInvariantMaintained(s:TaggedGLS_State, s':TaggedGLS_State)
-  requires SingleGLSPerformanceAssumption(s) && TGLS_Consistency(s)
-  requires SingleGLSPerformanceAssumption(s') && TGLS_Consistency(s')
-  requires TGLS_Next(s, s')
-  requires PerfInvariant(s)
-
-  ensures PerfInvariant(s')
-{
-  if (exists j, epoch :: 0 < epoch <= |s.tls.config| && epoch == j + 1 && 0 <= j < |s.tls.config| && PerfInvariantLockHeld(s, j, epoch)) {
-    var epoch, j :| 0 < epoch <= |s.tls.config| && epoch == j + 1 && 0 <= j < |s.tls.config| && PerfInvariantLockHeld(s, j, epoch);
-    PerfInvariantLockHeldGoesToPerfInvariant(j, epoch, s, s');
-  }
-  else {
-    var epoch, j :| 1 < epoch <= |s.tls.config| && epoch == j + 1 && 0 <= j < |s.tls.config| && PerfInvariantLockInNetwork(s, j, epoch);
-    PerfInvariantLockInNetworkGoesToPerfInvariant(j, epoch, s, s');
-  }
-}
-
-lemma {:verify false} Establish_TGLS_Consistency(config:Config, tglb:seq<TaggedGLS_State>, i:int)
-  requires ValidTaggedGLSBehavior(tglb, config)
-  requires 0 <= i < |tglb|
-  ensures TGLS_Consistency(tglb[i])
-
-  decreases i
-{
-  if i > 0{
-    Establish_TGLS_Consistency(config, tglb, i - 1);
-  }
-}
-
-lemma {:verify false} InitImpliesPerfInvariant(config:Config, s:TaggedGLS_State)
-  requires TGLS_Init(s, config)
-  requires TGLS_Consistency(s);
-  ensures PerfInvariant(s)
-{
-  //reveal_PerfInvariantLockHeld();
-  assert PerfInvariantLockHeld(s, 0, 1);
-}
-
-lemma {:verify false} PerfInvariantImpliesPerfGuarantee(s:TaggedGLS_State)
-  requires PerfInvariant(s)
-  ensures SingleGLSPerformanceGuarantee(s)
-{
-  //reveal_PerfInvariantLockHeld();
-  //reveal_PerfInvariantLockInNetwork();
-}
-
-lemma {:verify false} PerformanceGuaranteeHolds(config:Config, tglb:seq<TaggedGLS_State>)
-  requires ValidTaggedGLSBehavior(tglb, config)
-  requires GLSPerformanceAssumption(tglb)
-  ensures GLSPerformanceGuarantee(tglb)
-{
-  var i := 0;
-  Establish_TGLS_Consistency(config, tglb, 0);
-  InitImpliesPerfInvariant(config, tglb[0]);
-
-  while i < |tglb| - 1
-    invariant 0 <= i < |tglb|
-    invariant GLSPerformanceGuarantee(tglb[..i+1])
-    invariant PerfInvariant(tglb[i])
-  {
-    Establish_TGLS_Consistency(config, tglb, i);
-    Establish_TGLS_Consistency(config, tglb, i + 1);
-    PerfInvariantMaintained(tglb[i], tglb[i + 1]);
-    PerfInvariantImpliesPerfGuarantee(tglb[i+1]);
-    i := i + 1;
-  }
-}
 
 }
